\documentclass[../../HW02.tex]{subfiles}

\begin{document}
\begin{enumerate}
    \item Find the Fourier series of $f$ over $\left( -\pi,\pi \right)$. \label{1:a}
          \begin{align*}
              a_0 & = \frac{1}{2\pi}\int_{-\pi}^{\pi}f(x)\,dx          \\
              a_0 & = \frac{1}{\pi} \int_{0}^{\pi}x^2\,dx              \\
              a_0 & = \frac{1}{\pi} \left[ \frac{x^3}{3} \right]_0^\pi \\
              a_0 & = \frac{\pi^3}{3\pi}                               \\
              a_0 & =  \frac{\pi^2}{3}
          \end{align*}
          \begin{align*}
              a_n & = \frac{1}{\pi}\int_{-\pi}^{\pi} f(x)\cos(nx)\,dx                                                              \\
              a_n & = \frac{2}{\pi} \int_{0}^{\pi} x^2\cos(nx)\,dx                                                                 \\
              a_n & = \frac{2}{\pi} \left[ \frac{x^2}{n} \sin(nx) + \frac{2x}{n^2} \cos(nx) - \frac{2}{n^3} \sin(nx) \right]_0^\pi \\
              a_n & = \frac{2}{\pi} \left[ \frac{2\pi}{n^2} \cos(n\pi) - 0 \right]                                                 \\
              a_n & = \frac{2}{\pi} \left[ \frac{2\pi(-1)^n}{n^2} \right]                                                          \\
              a_n & = \frac{4(-1)^n}{n^2}
          \end{align*}
          \begin{center}
              $
                  \boxed{f(x) = \frac{\pi^2}{3} + \sum_{n=1}^{\infty}\frac{4(-1)^n}{n^2}\cos(nx)}
              $
          \end{center}
    \item Using \ref{1:a}, show that $\frac{\pi}{12}=\sum_{n=1}^{\infty} \frac{\left( -1 \right)^{n+1}}{n^2}$.
          \begin{align*}
              f(0)              & = \frac{\pi^2}{3} + \sum_{n=1}^{\infty}\frac{4(-1)^n}{n^2}\cos(0) \\
              \frac{-\pi^2}{3}  & = 4 \sum_{n=1}^{\infty}\frac{(-1)^n}{n^2}                         \\
              \frac{-\pi^2}{12} & = \sum_{n=1}^{\infty}\frac{(-1)^n}{n^2}                           \\
              \frac{\pi^2}{12}  & = \sum_{n=1}^{\infty}\frac{(-1)^{n+1}}{n^2}
          \end{align*}
    \item Using \ref{1:a} and Parseval's identity, show that $\frac{\pi^4}{90}=\sum_{n=1}^{\infty}\frac{1}{n^4}$.
          \begin{align*}
              \frac{1}{2L}\int_{-L}^{L}\left| f(x) \right|^2       & = a_0^2 + \frac{1}{2}\sum_{n=1}^{\infty}\left( a_n^2+b_n^2 \right)                                      \\
              \frac{1}{2\pi} \int_{-\pi}^{\pi}\left| x^2 \right|^2 & = \left( \frac{\pi^2}{3} \right)^2 + \frac{1}{2}\sum_{n=1}^{\infty}\left( \frac{4(-1)^n}{n^2} \right)^2 \\
              \text{LHS}                                           & = \frac{1}{\pi}\int_{0}^{\pi}x^4\,dx                                                                    \\
                                                                   & = \frac{1}{\pi}\left[ \frac{x^5}{5} \right]_0^\pi                                                       \\
                                                                   & = \frac{\pi^4}{5}                                                                                       \\
              \text{RHS}                                           & = \left( \frac{\pi^2}{3} \right)^2 + \frac{1}{2}\sum_{n=1}^{\infty}\left( \frac{4(-1)^n}{n^2} \right)^2 \\
                                                                   & = \frac{\pi^4}{9} + \frac{1}{2}\sum_{n=1}^{\infty}\frac{16}{n^4}                                        \\
                                                                   & = \frac{\pi^4}{9} + 8 \sum_{n=1}^{\infty}\frac{1}{n^4}                                                  \\
              \\
              \frac{\pi^4}{5}                                      & = \frac{\pi^4}{9} + 8\sum_{n=1}^{\infty} \frac{1}{n^4}                                                  \\
              \pi^4 \left( \frac{1}{5} - \frac{1}{9} \right)       & = 8\sum_{n=1}^{\infty} \frac{1}{n^4}                                                                    \\
              \frac{4\pi^4}{45}                                    & = 8\sum_{n=1}^{\infty} \frac{1}{n^4}                                                                    \\
              \frac{\pi^4}{90}                                     & = \sum_{n=1}^{\infty} \frac{1}{n^4}
          \end{align*}
\end{enumerate}
\end{document}