\documentclass[../../HW02.tex]{subfiles}

\begin{document}
\begin{align*}
    f(x)       & = \int_{0}^{\infty}A(\lambda)\cos(\lambda x) + B(\lambda)\sin(\lambda x)\,d\lambda                                                                                            \\
    A(\lambda) & = \int_{-\infty}^{\infty}f(x)\cos(\lambda x)\,dx                                                                                                                              \\
    A(\lambda) & = 2 \int_{0}^{\pi}\sin(x)\cos(\lambda x)\,dx                                                                                                                                  \\
    A(\lambda) & = 2 \int_{0}^{\pi} \frac{1}{2} \left[ \sin(x(1+\lambda)) + \sin(x(1-\lambda)) \right]\,dx                                                                                     \\
    A(\lambda) & = \left. \frac{-\cos(x (1+\lambda))}{1+\lambda} + \frac{-\cos(x(1-\lambda))}{1-\lambda}\right|_0^\pi                                                                          \\
    A(\lambda) & = \frac{-\cos(\pi(1+\lambda))}{1+\lambda} + \frac{\cos(\pi(1-\lambda))}{1-\lambda} + \frac{\cancelto{1}{\cos(0)}}{1+\lambda} + \frac{\cancelto{1}{\cos(0)}}{1-\lambda}        \\
    A(\lambda) & = \frac{\cos(\lambda\pi)}{1 + \lambda} + \frac{\cos(\lambda \pi)}{1 - \lambda} + \frac{1}{1 + \lambda} + \frac{1}{1 - \lambda}                                                \\
    A(\lambda) & = \frac{1 + \cos(\lambda\pi)}{1 + \lambda} + \frac{1 + \cos(\lambda \pi)}{1 - \lambda}                                                                                        \\
    A(\lambda) & = \frac{1 + \cos(\lambda\pi)}{1 - \lambda^2}                                                                                                                                  \\
    B(\lambda) & = \int_{-\infty}^{\infty} f(x)\sin(\lambda x)\,dx                                                                                                                             \\
    B(\lambda) & = 2 \int_{0}^{\pi}\sin(x)\sin(\lambda x)\,dx                                                                                                                                  \\
    B(\lambda) & = \int_{0}^{\pi} \cos(x(1-\lambda)) - \cos(x(1+\lambda))\,dx                                                                                                                  \\
    B(\lambda) & = \left. \frac{\sin(x(1-\lambda))}{1-\lambda} - \frac{\sin(x(1+\lambda))}{1+\lambda}\right|_0^\pi                                                                             \\
    B(\lambda) & = \frac{\sin(\pi(1-\lambda))}{1-\lambda} - \frac{\sin(\pi(1+\lambda))}{1+\lambda}                                                                                             \\
    B(\lambda) & = \frac{\sin(\lambda \pi)}{1 - \lambda} - \frac{\sin(\lambda \pi)}{1 + \lambda}                                                                                               \\
    B(\lambda) & = \sin(\lambda\pi)\left[ \frac{1}{1-\lambda} - \frac{1}{1+\lambda} \right]                                                                                                    \\
    B(\lambda) & = \sin(\lambda\pi) \left[ \frac{(1 + \lambda) - (1-\lambda)}{1 - \lambda^2} \right]                                                                                           \\
    B(\lambda) & = \frac{2\lambda\sin(\lambda\pi)}{1 - \lambda^2}                                                                                                                              \\
    f(x)       & = \boxed{\frac{1}{\pi} \int_{0}^{\infty} \frac{1 + \cos(\lambda\pi)}{1 - \lambda^2}\cos(\lambda x) + \frac{2\lambda\sin(\lambda\pi)}{1 - \lambda^2}\sin(\lambda x)\,d\lambda}
\end{align*}
\end{document}