\documentclass[../../HW02.tex]{subfiles}

\begin{document}
\begin{enumerate}
    \item Find the Fourier series of $f(x)$ over $\left( -\pi,\pi \right)$. \label{2:a}
          \begin{align*}
              a_0 & = \frac{1}{2\pi}\int_{-\pi}^{\pi}f(x)\,dx     \\
              a_0 & = \frac{1}{2\pi}\int_{0}^{\pi}\sin(x)\,dx     \\
              a_0 & = \frac{1}{2\pi}\left[ -\cos(x) \right]_0^\pi \\
              a_0 & = \frac{1}{2\pi}\left[ -(-1) - (-1) \right]   \\
              a_0 & = \frac{1}{\pi}                               \\
          \end{align*}
          \begin{align*}
              a_n & = \frac{1}{\pi}\int_{-\pi}^{\pi}f(x)\cos(nx)\,dx                                                                                                                                     \\
              a_n & = \frac{1}{\pi}\int_{0}^{\pi} \sin(x)\cos(nx)\,dx                                                                                                                                    \\
              a_n & = \frac{1}{\pi}\int_{0}^{\pi} \frac{1}{2} \left[ \sin\left( (n+1)x \right) - \sin\left( (n-1) x \right) \right]\,dx                                                                  \\
              a_n & = \frac{1}{2\pi} \left[ \frac{-\cos\left( (n+1) x \right)}{n+1} + \frac{\cos \left( (n-1) x \right)}{n-1} \right]_0^\pi                                                              \\
              a_n & = \frac{1}{2\pi} \left[ \left( \frac{-\cos\left( (n+1) \pi \right)}{n+1} + \frac{\cos \left( (n-1) \pi \right)}{n-1} \right) - \left( \frac{-1}{n+1} + \frac{1}{n-1} \right) \right] \\
              a_n & = \frac{1}{2\pi} \left[ \frac{(-1)^n}{n+1} + \frac{-(-1)^n}{n-1} + \frac{1}{n+1} + \frac{-1}{n-1} \right]                                                                            \\
              a_n & = \frac{1}{2\pi} \left[ \frac{1+(-1)^n}{n+1} - \frac{1+(-1)^n}{n-1} \right]                                                                                                          \\
              a_n & = \frac{1+(-1)^n}{2\pi} \left[ \frac{-2}{n^2-1} \right]                                                                                                                              \\
              a_n & =
              \begin{cases}
                  0,                                    & \text{if $n$ is odd}  \\
                  \frac{-2}{\left( n^2 - 1\right) \pi}, & \text{if $n$ is even}
              \end{cases}
          \end{align*}
          \begin{align*}
              b_n              & = \frac{1}{\pi}\int_{-\pi}^{\pi}f(x)\sin(nx)\,dx                                                                           \\
              b_n              & = \frac{1}{\pi}\int_{0}^{\pi}\sin(x)\sin(nx)\,dx                                                                           \\
              b_n              & = \frac{1}{\pi}\int_{0}^{\pi}\frac{1}{2}\left[ \cos\left( (n-1) x \right) - \cos\left( (n+1) x \right) \right]\,dx         \\
              n=1\qquad b_1    & = \frac{1}{2\pi}\int_{0}^{\pi}1-\cos(2x)\,dx                                                                               \\
              b_1              & = \frac{1}{2\pi}\left[ x - \frac{\sin(2x)}{2} \right]_0^\pi                                                                \\
              b_1              & = \frac{1}{2}                                                                                                              \\
              n\ne1 \qquad b_n & = b_n = \frac{1}{2\pi}\left[ \frac{\sin\left( (n-1) x \right)}{n-1} - \frac{\sin\left( (n+1) x \right)}{n+1} \right]_0^\pi \\
              b_n              & = 0
          \end{align*}
          \begin{align*}
              f(x) & =\frac{1}{\pi} + \frac{1}{2}\sin(x) + \sum_{\text{$n$ = even}}^{\infty}\frac{-2}{(n^2 -1)\pi}\cos(nx)      \\
              f(x) & = \boxed{\frac{1}{\pi} + \frac{1}{2}\sin(x) + \frac{-2}{\pi}\sum_{n=1}^{\infty}\frac{\cos(2nx)}{(2n)^2-1}}
          \end{align*}
    \item Using \ref{2:a} and Parseval's identity, show that:
          \begin{center}
              $\frac{\pi^2}{16}-\frac{1}{2}=\sum_{\text{$k =$ even}}^{\infty}\frac{1}{\left( k^2 - 1 \right)^2}.$
          \end{center}
          \begin{align*}
              \frac{1}{2L} \int_{-L}^{L}\left| f(x) \right|^2\,dx & = a_0^2 + \frac{1}{2}\sum_{n=1}^{\infty}a_n^2+b_n^2                                                              \\
              \text{LHS:}                                         & = \frac{1}{2\pi} \int_{-\pi}^{\pi} \left| f(x) \right|^2                                                         \\
                                                                  & = \frac{1}{2\pi} \int_{0}^{\pi} \sin^2(x)\,dx                                                                    \\
                                                                  & = \frac{1}{2\pi} \int_{0}^{\pi} \frac{1-\cos(2x)}{2}\,dx                                                         \\
                                                                  & = \frac{1}{4\pi} \int_{0}^{\pi} 1 - \cos(2x) \,dx                                                                \\
                                                                  & = \frac{1}{4\pi} \left[ x - \frac{\sin(2x)}{2} \right]_0^\pi                                                     \\
                                                                  & = \frac{1}{4\pi} \left[ \left( \pi - \frac{\sin(2\pi)}{2} \right) - \left( 0 - \frac{\sin(0)}{2} \right) \right] \\
                                                                  & = \frac{1}{4\pi} \cdot \pi                                                                                       \\
                                                                  & = \frac{1}{4}                                                                                                    \\
              \text{RHS: }                                        & = a_0^2 + \frac{1}{2} \sum_{n=1}^{\infty}a_n^2+b_1^2                                                             \\
                                                                  & = \frac{1}{\pi^2} + \frac{1}{2}\sum_{n=1}^{\infty}\frac{4}{\left( (2n)^2 - 1 \right)^2 \pi^2} + \frac{1}{4}      \\
                                                                  & = \frac{1}{\pi^2} + \frac{1}{8} + \frac{2}{\pi^2}\sum_{n=1}^{\infty}\frac{1}{\left( (2n)^2 - 1 \right)^2}        \\
              \\
              \frac{1}{4}                                         & = \frac{1}{\pi^2} + \frac{1}{8} + \frac{2}{\pi^2}\sum_{n=1}^{\infty}\frac{1}{\left( (2n)^2 - 1 \right)^2}        \\
              \frac{1}{4} - \frac{1}{\pi^2} - \frac{1}{8}         & = \frac{2}{\pi^2} \sum_{n=1}^{\infty} \frac{1}{\left( (2n)^2 - 1 \right)^2}                                      \\
              \frac{\pi^2 - 8}{8\pi^2}                            & = \frac{2}{\pi^2} \sum_{n=1}^{\infty} \frac{1}{\left( (2n)^2 - 1 \right)^2}                                      \\
              \frac{\pi^2 - 8}{16}                                & = \sum_{n=1}^{\infty} \frac{1}{\left( (2n)^2 - 1 \right)^2}                                                      \\
              \frac{\pi^2}{16} - \frac{1}{2}                      & = \sum_{\text{$k$ = even}}^{\infty} \frac{1}{(k^2 - 1)^2}
          \end{align*}
\end{enumerate}
\end{document}